Add support for definitions (views) in OQL.  Change oql type to be that of a oql program (with definitions).  Fixup semantics, typing, translation to NRAenv and proofs.

coq/Compiler/CompilerDriver/CompLang.v
@@ -46,7 +46,7 @@ Section CompLang.
 
   Definition rule := rule.
   Definition camp := pat.
-  Definition oql := oql_expr.
+  Definition oql := oql.
   Definition sql := sql.
   Definition lambda_nra := lalg.
   Definition nra := alg.
